src/named/PfCore.v
@@ -1,0 +1,718 @@
+Require Import mathcomp.ssreflect.all_ssreflect.
+Set Implicit Arguments.
+Unset Strict Implicit.
+Unset Printing Implicit Defensive.
+Set Bullet Behavior "Strict Subproofs".
+
+From Utils Require Import Utils.
+From Named Require Import Pf.
+
+Require Import String.
+
+
+Create HintDb pfcore discriminated.
+
+
+
+(*TODO: put in utils*)
+Lemma in_all_fresh_same {A:eqType} (a b : A) l s
+  : all_fresh l -> (s,a) \in l -> (s,b) \in l -> a = b.
+Proof.
+  induction l; simpl; intros; break;
+    repeat match goal with
+           | [H : is_true (_\in [::])|- _] =>
+             solve[ inversion H]
+           | [H : is_true (_\in _::_)|- _] =>
+             rewrite in_cons in H;
+               move: H => /orP []; intros; break
+           | [H : is_true ((_,_) == (_,_))|- _] =>
+             move: H => /eqP []; intros; subst
+           end; simpl in *; auto.
+  eapply fresh_neq_in in H2; eauto;
+  exfalso;  move: H2 => /eqP; auto.
+  eapply fresh_neq_in in H2; eauto;
+  exfalso;  move: H2 => /eqP; auto.
+Qed.
+
+
+Lemma named_list_lookup_none {A:eqType} l s (a:A)
+  : None = named_list_lookup_err l s ->
+    (s, a) \notin l.
+Proof.
+  induction l; break; simpl in *; auto.
+  case seqs0: (s=?s0)%string.
+  {
+    intro fls; inversion fls.
+  }
+  {
+    intros; rewrite in_cons; apply /orP.
+    intro c; destruct c.
+    {
+      cbn in *.
+      rewrite seqs0 in H0; move: H0 => /andP [] //.
+    }
+    {
+      apply IHl in H.
+      rewrite H0 in H.
+      inversion H.
+    }
+  }
+Qed.
+  
+Section TermsAndRules.
+  Context (l : pf_lang).
+
+  (*TODO: rename these to dom and codom? *)
+  (*Pressupposition: p is ok *)
+  Fixpoint proj_l (p:pf) :=
+    match p with
+    | pvar x => (pvar x)
+    | pcon name pl => pcon name (map proj_l pl)
+    | ax name pl =>
+      match named_list_lookup_err l name with
+      | Some (sort_le_pf c p' _)
+      | Some (term_le_pf c p' _ _) =>
+        pf_subst (with_names_from c (map (proj_l) pl)) p'
+      | _ => pcon "ERR" [::]
+      end
+    | sym p => proj_r p
+    | trans p1 p2 => proj_l p1
+    | conv pt p' => conv pt (proj_l p')
+    end
+  (*Pressupposition: p is ok *)
+  with proj_r (p:pf) :=
+    match p with
+    | pvar x => (pvar x)
+    | pcon name pl => pcon name (map proj_l pl)
+    | ax name pl =>
+      match named_list_lookup_err l name with
+      | Some (sort_le_pf c _ p')
+      | Some (term_le_pf c _ p' _) =>
+        pf_subst (with_names_from c (map (proj_l) pl)) p'
+      | _ => pcon "ERR" [::]
+      end
+    | sym p => proj_l p
+    | trans p1 p2 => proj_r p2
+    | conv pt p' => conv pt (proj_l p')
+    end.
+
+  (* Strips components of the proof that we consider
+     irrelevant for the purpose of equality.
+     TODO: generalize this, e.g. (sym (sym x)) ~ x.
+     Probably not necessary as long as this is only
+     used on projections
+   *)
+  Fixpoint strip_irrelevant (e : pf) : pf :=
+    match e with
+    | pvar x => (pvar x)
+    | pcon name pl => 
+      match named_list_lookup_err l name with
+      | Some (sort_rule_pf c args)
+      | Some (term_rule_pf c args _) =>
+        match get_subseq args (with_names_from c (map (proj_l) pl)) with
+        | Some pl' => pcon name (map snd pl')
+        | None => pcon "ERR" [::]
+        end
+      | _ => pcon name (map strip_irrelevant pl)
+      end
+    | ax name pl => ax name (map strip_irrelevant pl)
+    | sym p => sym (strip_irrelevant p)
+    | trans p1 p2 => trans (strip_irrelevant p1) (strip_irrelevant p2)
+    | conv _ p' => (strip_irrelevant p')
+    end.
+
+  (* TODO: this is a shortcut; it's probably safe but should
+     be generalized at some point.
+     Current potential issues: 
+     -sym, trans in sorts
+     Should definitely be safe when used on projections
+
+    TODO: define (proj_l a `eq_pf_irr` proj_r b) as a
+    relation for ease-of-proof?
+   *)
+  Definition eq_pf_irr (e1 e2 : pf): bool :=
+    (strip_irrelevant e1) == (strip_irrelevant e2).
+  
+  (*
+    Judgments for checking proofs of relations between programs.
+    Can check wfness of a program by identifying it with its
+    identity relation.
+
+    All assume lang_ok.
+    All ctxs (other than in ctx_ok) are assumed to satisfy ctx_ok.
+    Judgments whose assumptions take ctxs must ensure they are ok.
+    Sorts are not assumed to be ok; the term judgments should guarantee
+    that their sorts are ok.
+   *)
+  
+  Inductive sort_ok : pf_ctx -> pf -> Prop :=
+  | sort_ok_ax : forall c c' name t1 t2 s,
+      (name, sort_le_pf c' t1 t2) \in l ->
+      args_ok c s c' ->
+      sort_ok c (ax name s)
+  | sort_ok_con : forall c name c' args s,
+      (name, (sort_rule_pf c' args)) \in l ->
+      args_ok c s c' ->
+      sort_ok c (pcon name s)
+  | sort_ok_trans : forall c t1 t2,
+      sort_ok c t1 ->
+      sort_ok c t2 ->
+      eq_pf_irr (proj_r t1) (proj_l t2) ->
+      sort_ok c (trans t1 t2)
+  | sort_ok_sym : forall c t, sort_ok c t -> sort_ok c (sym t)
+  with term_ok : pf_ctx -> pf -> pf -> Prop :=
+  | term_ok_ax : forall c c' name e1 e2 t s,
+      (name, term_le_pf c' e1 e2 t) \in l ->
+      args_ok c s c' ->
+      (*non-obvious fact: the sort may not be a wfness proof;
+        may be a non-identity relation due to s
+       *)
+      term_ok c (ax name s) (pf_subst (with_names_from c' s) t)
+  | term_ok_con : forall c name c' args t s,
+      (name, (term_rule_pf c' args t)) \in l ->
+      args_ok c s c' ->
+      (* same as above *)
+      term_ok c (pcon name s) (pf_subst (with_names_from c' s) t)
+  | term_ok_trans : forall c e1 t1 e2 t2,
+      term_ok c e1 t1 ->
+      term_ok c e2 t2 ->
+      eq_pf_irr (proj_r e1) (proj_l e2) ->
+      eq_pf_irr (proj_r t1) (proj_l t2) ->
+      term_ok c (trans e1 e2) (trans t1 t2)
+  | term_ok_sym : forall c e t, term_ok c e t -> term_ok c (sym e) (sym t)
+  | term_ok_var : forall c x t,
+      (x,t) \in c ->
+      term_ok c (pvar x) t
+  (* Conversion:
+
+c |- e1 = e2 : t = t'
+                 ||
+c |- e1 = e2 : t' = t''
+   *)
+  | term_ok_conv : forall c e t t',
+      sort_ok c t' ->
+      term_ok c e t ->
+      eq_pf_irr (proj_r t) (proj_l t') ->
+      term_ok c (conv t' e) (trans t t')
+  with args_ok : pf_ctx -> list pf -> pf_ctx -> Prop :=
+  | args_ok_nil : forall c, args_ok c [::] [::]
+  | args_ok_cons : forall c s c' name e t,
+      args_ok c s c' ->
+      (* assumed because the output ctx is wf: fresh name c' ->*)
+      term_ok c e (pf_subst (with_names_from c' s) t) ->
+      args_ok c (e::s) ((name, t)::c').
+  
+  Inductive subst_ok : pf_ctx -> named_list pf -> pf_ctx -> Prop :=
+  | subst_ok_nil : forall c, subst_ok c [::] [::]
+  | subst_ok_cons : forall c s c' name e t,
+      subst_ok c s c' ->
+      (* assumed because the output ctx is wf: fresh name c' ->*)
+      term_ok c e (pf_subst s t) ->
+      subst_ok c ((name,e)::s) ((name, t)::c').
+
+  Inductive ctx_ok : pf_ctx -> Prop :=
+  | ctx_ok_nil : ctx_ok [::]
+  | ctx_ok_cons : forall name c v,
+      fresh name c ->
+      ctx_ok c ->
+      sort_ok c v ->
+      ctx_ok ((name,v)::c).
+
+  (* Denotes when a proof represents
+     an expression (as opposed to a relation
+     between 2 expressions)
+   *)
+  Inductive is_exp : pf -> Prop :=
+  | var_is_exp x : is_exp (pvar x)
+  | con_is_exp name s
+    : List.Forall is_exp s ->
+      is_exp (pcon name s)
+  | conv_is_exp pt p
+    : is_exp p ->
+      is_exp (conv pt p).
+
+  Fixpoint check_is_exp e : bool :=
+    match e with
+    | pvar _ => true
+    | pcon _ s => List.forallb check_is_exp s
+    | conv _ p => check_is_exp p
+    | _ => false
+    end.
+
+  Lemma check_is_expP e : reflect (is_exp e) (check_is_exp e).
+  Proof using.
+    induction e; simpl; repeat constructor;
+    try match goal with
+        [|- ~_] => let H := fresh in intro H; inversion H; clear H; subst
+        end.
+    {
+      suff: (reflect (List.Forall is_exp l0) (List.forallb check_is_exp l0)).
+      {
+        intro lfr.
+        match goal with
+           |- reflect _ ?b =>
+           case alll0: b
+        end; repeat constructor.
+        { apply /lfr; assumption. }
+        {
+          intro H; inversion H; subst; clear H.
+          move: H1 => /lfr.
+          rewrite alll0 => //.
+        }
+      }
+      {
+        revert X; induction l0; simpl; [repeat constructor|].
+        intro; break.
+        solve_reflect_norec;
+          [match goal with
+             |- reflect _ ?b =>
+             case alll0: b
+           end|]; repeat constructor.
+        { apply /r; auto. }
+        { apply /IHl0; auto. }
+        {
+          intro H; inversion H; subst; clear H.
+          move: H3 => /IHl0.
+          rewrite alll0 => //.
+          auto.
+        }
+        {
+          intro H; inversion H; subst; clear H.
+          move: H2 => /r //.
+        }
+      }
+    }
+    {
+      revert IHe2.
+      case ce2: (check_is_exp e2); intro r; constructor; inversion r.
+      constructor; auto.
+      intro H'; inversion H'; auto.
+    }
+  Qed.  
+
+  (*TODO: for le's, how to make this
+    correspond to existing fwk; should I?
+    existing defs allow for higher rels in an unfortunate way.
+    e.g:
+    
+    ...
+    --------------------------------------------------
+    stlc_beta G A A' e e' = ... : (G |- A) = (G' |- B)
+    
+    where l[stlc_beta] = ...|- \e e' = e[/e'/]
+   *)
+  Variant rule_ok : rule_pf -> Prop :=
+  | sort_rule_ok : forall c args,
+      ctx_ok c ->
+      subseq args (map fst c) ->
+      rule_ok (sort_rule_pf c args)
+  | term_rule_ok : forall c args t,
+      ctx_ok c ->
+      sort_ok c t ->
+      subseq args (map fst c) ->
+      rule_ok (term_rule_pf c args t)
+  | sort_le_ok : forall c t1 t2,
+      ctx_ok c ->
+      is_exp t1 ->
+      is_exp t2 ->
+      sort_ok c t1 ->
+      sort_ok c t2 ->
+      rule_ok (sort_le_pf c t1 t2)
+  | term_le_ok : forall c e1 e2 t,
+      ctx_ok c ->
+      is_exp e1 ->
+      is_exp e2 ->
+      is_exp t ->
+      sort_ok c t ->
+      term_ok c e1 t ->
+      term_ok c e2 t ->
+      rule_ok (term_le_pf c e1 e2 t).
+
+  Hint Constructors sort_ok term_ok subst_ok args_ok ctx_ok rule_ok : pfcore.
+  
+  Section InnerLoop.
+    Context (check_term_ok : pf -> pf -> bool).
+    Context (lfresh : all_fresh l).
+    Context c (check_term_okP : forall e t, reflect (term_ok c e t) (check_term_ok e t)).
+
+    Fixpoint check_args_ok' (pl : list pf) (c' : pf_ctx) {struct pl} : bool :=
+      match pl, c' with
+      | [::], [::] => true
+      | p::pl', (_,t)::c'' =>
+        (check_term_ok p (pf_subst (with_names_from c'' pl') t)) &&
+        (check_args_ok' pl' c'')
+      |_,_=> false
+    end.
+
+    Fixpoint check_sort_ok' (pt : pf) : bool :=
+      match pt with
+      | pcon name pl =>
+        match named_list_lookup_err l name with
+        | Some (sort_rule_pf c' _) => check_args_ok' pl c'
+        | _ => false
+        end
+      | ax name pl =>
+        match named_list_lookup_err l name with
+        | Some (sort_le_pf c' _ _) => check_args_ok' pl c'
+        | _ => false
+        end
+      | sym p => check_sort_ok' p
+      | trans p1 p2 =>
+        (check_sort_ok' p1) &&
+        (check_sort_ok' p2) &&
+        (eq_pf_irr (proj_r p1) (proj_l p2))
+      | conv _ _ => false
+      | pvar _ => false
+      end.
+
+    Hint Constructors reflect : pfcore.
+         
+  End InnerLoop.
+
+  Fixpoint check_term_ok (c : pf_ctx) e t {struct e} : bool :=
+    match e with
+    | pvar x =>
+      match named_list_lookup_err c x with
+      | Some t' => t == t' (*TODO: this lines up w/ the inductive, 
+                             but maybe should be pf_eq_irr?
+                             Might want to change the inductive.
+                             Can be worked around w/ extra convs as is,
+                             but that might be easier.
+                             Same for other cases.
+                            *)
+      | None => false
+      end
+    | pcon name pl =>
+      match named_list_lookup_err l name with
+      | Some (term_rule_pf c' _ t') =>
+        (check_args_ok' (check_term_ok c) pl c') &&
+        (t == pf_subst (with_names_from c' pl) t')
+      | _ => false
+      end
+    | ax name pl =>
+      match named_list_lookup_err l name with
+      | Some (term_le_pf c' _ _ t') => 
+        (check_args_ok' (check_term_ok c) pl c') &&
+        (t == pf_subst (with_names_from c' pl) t')
+      | _ => false
+      end
+    | sym p =>
+      match t with
+      | sym t' => check_term_ok c p t'
+      | _ => false (*TODO: same thing as ==s above.
+                     This works, but it feels like I should use a looser
+                     defn of equivalence. Should come back to these if it
+                     ends up as a pain point.
+                    *)
+      end
+    | trans p1 p2 => 
+      match t with
+      | trans t1 t2 =>
+        (check_term_ok c p1 t1) &&
+        (check_term_ok c p2 t2) &&
+        (eq_pf_irr (proj_r p1) (proj_l p2)) &&
+        (eq_pf_irr (proj_r t1) (proj_l t2))
+      | _ => false (*TODO: same thing as ==s above.
+                     This works, but it feels like I should use a looser
+                     defn of equivalence. Should come back to these if it
+                     ends up as a pain point.
+                    *)
+      end
+    | conv pt p' =>
+      match t with
+      | trans t1 t2 =>
+      (pt == t2) &&
+      (eq_pf_irr (proj_r t1) (proj_l t2)) &&
+      (check_sort_ok' (check_term_ok c) pt) &&
+      (check_term_ok  c p' t1)
+      | _ => false (*TODO: same thing as ==s above.
+                     This works, but it feels like I should use a looser
+                     defn of equivalence. Should come back to these if it
+                     ends up as a pain point.
+                    *)
+      end
+    end.
+
+  
+  (*TODO: build right induction*)
+  Lemma check_term_okP c e t
+    : all_fresh l ->
+      all_fresh c ->
+      reflect (term_ok c e t) (check_term_ok c e t)
+  with check_args_ok'P c pl c'
+       : all_fresh l ->
+         all_fresh c ->
+         reflect (args_ok c pl c') (check_args_ok' (check_term_ok c) pl c')
+  with check_sort_ok'P c t
+      : all_fresh l ->
+        all_fresh c ->
+        reflect (sort_ok c t) (check_sort_ok' (check_term_ok c) t).
+  Proof using.
+    all: intros frl frc.
+    all: match goal with
+    | [|- reflect (term_ok _ ?e _) _]=> destruct e
+    | [|- reflect (sort_ok _ ?t) _]=> destruct t
+    | [|- reflect (args_ok _ ?s _) _]=> destruct s
+    end; intros; repeat (break; simpl in *; try case_match);
+      repeat lazymatch goal with
+    | [|- args_ok _ [::] [::]] => by constructor
+    | [|- args_ok _ (_::_) (_::_)] => constructor
+    | [|- sort_ok _ (sym _)] => apply sort_ok_sym
+    | [|- sort_ok _ (trans _ _)] => apply sort_ok_trans
+     (*Recursive cases; proceed w/ caution*)
+    | [H : is_true(check_term_ok _ ?e ?t) |- term_ok _ ?e ?t]=>
+      apply /check_term_okP; auto
+    | [H : is_true(check_args_ok' _ ?e ?t) |- args_ok _ ?e ?t]=>
+      apply /check_args_ok'P; auto
+    | [H : is_true(check_sort_ok' _ ?t) |- sort_ok _ ?t]=>
+      apply /check_sort_ok'P; auto
+    (* end of recursive cases *)
+    | [ H: ?P |- ?P] => exact H
+    | [ H: ?P, Hf : ~?P |- _] => exfalso; exact (Hf H)
+    | [|- is_true(?a == ?a)]=> apply /eqP
+    | [H : ~(is_true(?a == ?a)) |-_]=>
+      exfalso; exact (H (eq_refl a))
+    | [|- ?a = ?a]=> reflexivity
+    | [H : term_le_pf _ _ _ _ = _ |-_]=> inversion H; subst; clear H
+    | [H : sort_le_pf _ _ _ = _ |-_]=> inversion H; subst; clear H
+    | [H : sort_rule_pf _ _ = _ |-_]=> inversion H; subst; clear H
+    | [H : term_rule_pf _ _ _ = _ |-_]=> inversion H; subst; clear H
+    | [H : true = true |-_]=> clear H
+    | [H : true = ?a |-_]=> symmetry in H
+    | [H : (?a)=true |-_]=> change (is_true a) in H
+    | [H : false = false |-_]=> clear H
+    | [H : false = ?a |-_]=> symmetry in H
+    | [H : is_true(_&&_) |-_]=> break
+    | [|-is_true(_&&_)]=> break_goal
+    | [H : is_true(_==_) |-_]=> move: H => /eqP H; subst
+    | [H : (?e==?e)=false |-_]=> rewrite eq_refl in H; inversion H
+    | [H : ?a = false, H': is_true ?a |-_]=> rewrite H in H'; inversion H'
+    | [|- reflect _ true]=> constructor
+    | [|- reflect _ false]=> constructor
+    | [|- reflect _ ?p]=>
+      let H := fresh in my_case H p
+    | [|- ~_]=> let H:= fresh in intro H; inversion H; subst; clear H; auto
+    |[_:~_, _:~_|-_] => idtac "two possible negations"
+    |[H:~_|-False] => apply H 
+    | [|- rule_ok _]=> constructor; auto
+    | [|- term_ok _ _ _]=> constructor
+    | [|- ctx_ok _]=> apply /check_ctx_okP; auto
+    | [H : ~(is_true(check_args_ok' _ ?e ?t)), H' : args_ok _ ?e ?t|- _]=>
+      move: H => /negP /check_args_ok'P H;
+      exfalso; apply H; auto
+    | [H : ~(is_true(check_term_ok _ ?e ?t)), H' : term_ok _ ?e ?t|- _]=>
+      move: H => /negP /check_term_okP H;
+      exfalso; apply H; auto
+    | [H : ~(is_true(check_sort_ok' _ ?t)), H' : sort_ok _ ?t|- _]=>
+      move: H => /negP /check_sort_ok'P H;
+      exfalso; apply H; auto
+    | [H : check_term_ok _ ?e ?t = false, H' : term_ok _ ?e ?t|- _]=>
+      move: H' => /check_term_okP; rewrite H; auto
+    | [H : check_args_ok' _ ?e ?t = false, H' : args_ok _ ?e ?t|- _]=>
+      move: H' => /check_args_ok'P; rewrite H; auto
+    | [H : check_sort_ok' _ ?t = false, H' : sort_ok _ ?t|- _]=>
+      move: H' => /check_sort_ok'P; rewrite H; auto
+    | [H : check_is_exp ?e = false, H' : is_exp ?e|- _]=>
+      move: H' => /check_is_expP; rewrite H; auto
+    | [|- is_exp _]=> apply /check_is_expP; auto
+    | [|- is_true (_\in_)]=> by apply named_list_lookup_err_in
+    | [H: Some _ = named_list_lookup_err _ _|- _]=>
+      apply named_list_lookup_err_in in H
+    | [H1 : is_true((?n,?a)\in ?l),
+       H2 : is_true((?n,?b)\in ?l),
+       Hfr : is_true(all_notin (map fst ?l))
+                       |- _]=>
+      let H' := fresh in
+      pose proof (in_all_fresh_same Hfr H1 H2) as H';
+        clear H2;
+        move: H' => /eqP H'; subst
+    | [H: None = named_list_lookup_err _ ?n,
+       H' : is_true((?n,_)\in _) |- _]=>
+      eapply named_list_lookup_none in H;
+      erewrite H' in H; simpl in H; inversion H
+    | [H: ~(is_true(_&&_)) |-_]=>
+       move: H => /negP /nandP [] H
+    | [H: (_&&_)=false |-_]=>
+       move: H => /nandP [] H
+    |[H:is_true(~~_)|-_] => move: H => /negP H
+             end.
+    { (*TODO: automate*)
+      eapply term_ok_con.
+      apply named_list_lookup_err_in; eauto.
+      apply /check_args_ok'P; auto.
+    }
+    { (*TODO: automate*)
+      eapply term_ok_ax.
+      apply named_list_lookup_err_in; eauto.
+      apply /check_args_ok'P; auto.
+    }
+    { (*TODO: automate*)
+      eapply sort_ok_con; eauto.
+      apply /check_args_ok'P; auto.
+    }
+    { (*TODO: automate*)
+      eapply sort_ok_ax; eauto.
+      apply /check_args_ok'P; auto.
+    }
+   (* TODO: break 2 directions up to make the fixpoint go through?
+                reflection harder to reason about wrt termination
+      prob not necessary w/ right recursion*)
+    (*Guarded.*)
+  Admitted.
+
+  Definition check_sort_ok c t := check_sort_ok' (check_term_ok c) t.
+  Definition check_args_ok c s c' := check_args_ok' (check_term_ok c) s c'.
+
+  
+  Lemma check_sort_okP c t
+      : all_fresh l -> all_fresh c -> reflect (sort_ok c t) (check_sort_ok c t).
+  Proof using.
+    eauto using check_term_okP, check_sort_ok'P.
+  Qed.
+
+  
+  Lemma check_args_okP c s c'
+    : all_fresh l -> all_fresh c ->
+      reflect (args_ok c s c') (check_args_ok c s c').
+  Proof using.
+    eauto using check_term_okP, check_args_ok'P.
+  Qed.
+
+  Fixpoint check_ctx_ok c :=
+    match c with
+    | [::] => true
+    | (name,t)::c' =>
+      (fresh name c') &&
+      (check_sort_ok c' t) &&
+      (check_ctx_ok c')
+    end.
+
+  
+  Lemma ctx_ok_all_fresh c
+    : ctx_ok c -> all_fresh c.
+  Proof using.
+    induction c; intro cok; inversion cok; subst; clear cok; break; simpl in *;
+      break_goal; auto.
+  Qed.
+  Hint Resolve ctx_ok_all_fresh : pfcore.
+
+  Lemma check_ctx_okP c : all_fresh l -> reflect (ctx_ok c) (check_ctx_ok c).
+  Proof using.
+    intro frl.
+    induction c; intros; break; simpl; repeat constructor.
+    repeat lazymatch goal with
+           | [|- reflect _ (_&&_)]=>
+             (destruct_reflect_andb_l; simpl)
+           end.
+    lazymatch goal with
+    | [|- reflect _ ?p]=>
+      let H := fresh in my_case H p
+    end.
+    all: constructor.
+    {
+      constructor;
+      inversion IHc; auto.
+      apply /check_sort_okP; auto using ctx_ok_all_fresh.
+    }
+    all: intro cok; inversion cok; subst; clear cok.
+      match goal with
+        [ H : reflect _ false |-_]=> inversion H
+      end; auto using ctx_ok_all_fresh.
+      match goal with
+        [ frl : is_true(all_fresh l),
+          H : false = check_sort_ok ?c ?p,
+          H' : sort_ok ?c ?p |-_]=>
+        move: H' => /(check_sort_okP); intro H';
+        rewrite <-H in H'; auto using ctx_ok_all_fresh
+      end.
+      simpl in H2.
+      rewrite <-Heqb in H2; inversion H2.
+  Qed.
+    
+  Definition check_rule_ok r :=
+    match r with
+    | sort_rule_pf c args =>
+      (check_ctx_ok c) && (subseq args (map fst c))
+    | term_rule_pf c args t =>
+      (check_ctx_ok c) &&
+      (subseq args (map fst c)) &&
+      (check_sort_ok c t)
+    | sort_le_pf c t1 t2 =>
+      (check_ctx_ok c) &&
+      (check_is_exp t1) &&
+      (check_is_exp t2) &&
+      (check_sort_ok c t1) &&
+      (check_sort_ok c t2)
+    | term_le_pf c e1 e2 t =>
+      (check_ctx_ok c) &&
+      (check_is_exp e1) &&
+      (check_is_exp e2) &&
+      (check_is_exp t) &&
+      (check_term_ok c e1 t) &&
+      (check_term_ok c e2 t) &&
+      (check_sort_ok c t)
+    end.
+
+  Lemma check_rule_okP r : all_fresh l -> reflect (rule_ok r) (check_rule_ok r).
+  Proof using.
+    intro frl.
+    pose proof ctx_ok_all_fresh.
+    destruct r; intros; break; simpl; repeat constructor;
+    solve_reflect_norec;
+    repeat lazymatch goal with
+    | [H : true = true |-_]=> clear H
+    | [H : true = ?a |-_]=> symmetry in H
+    | [H : ?a=true |-_]=> change (is_true a) in H
+    | [H : false = false |-_]=> clear H
+    | [H : false = ?a |-_]=> symmetry in H
+    | [H : ?a = false, H': is_true ?a |-_]=> rewrite H in H'; inversion H'
+    | [|- reflect _ true]=> constructor
+    | [|- reflect _ false]=> constructor
+    | [|- reflect _ ?p]=>
+      let H := fresh in my_case H p
+    | [|- ~_]=> let H:= fresh in intro H; inversion H; subst; clear H; auto
+    | [|- rule_ok _]=> constructor; auto
+    | [|- term_ok _ _ _]=> apply /check_term_okP; auto
+    | [|- sort_ok _ _]=> apply /check_sort_okP; auto
+    | [|- ctx_ok _]=> apply /check_ctx_okP; auto
+    | [H : check_term_ok _ ?e ?t = false, H' : term_ok _ ?e ?t|- _]=>
+      move: H' => /check_term_okP; rewrite H; auto
+    | [H : check_sort_ok _ ?t = false, H' : sort_ok _ ?t|- _]=>
+      move: H' => /check_sort_okP; rewrite H; auto
+    | [H : check_ctx_ok _ = false, H' : ctx_ok _|- _]=>
+      move: H' => /check_ctx_okP; rewrite H; auto
+    | [H : check_is_exp ?e = false, H' : is_exp ?e|- _]=>
+      move: H' => /check_is_expP; rewrite H; auto
+    | [H : is_true(check_ctx_ok _)|- _]=>
+      move: H => /check_ctx_okP H
+    | [|- is_exp _]=> apply /check_is_expP; auto
+    end; auto.
+  Qed.
+  
+End TermsAndRules.
+
+
+Inductive lang_ok : pf_lang -> Prop :=
+| lang_ok_nil : lang_ok [::]
+| lang_ok_cons : forall name l r,
+    fresh name l ->
+    lang_ok l ->
+    rule_ok l r ->
+    lang_ok ((name,r)::l).
+
+
+Fixpoint check_lang_ok l :=
+    match l with
+    | [::] => true
+    | (name,r)::l' =>
+      (fresh name l') &&
+      (check_rule_ok l' r) &&
+      (check_lang_ok l')
+    end.
+
+
+Lemma check_lang_ok_all_fresh l : check_lang_ok l -> all_fresh l.
+Proof using.
+  induction l; intros; repeat (break; simpl in * ); break_goal; auto.
+Qed.  
+  
